Test/inline/codeexpr.bpl
@@ -5,6 +5,11 @@ procedure {:inline 1} bar() returns (l: bool)
   l := g;
 }
 
+procedure {:inline 1} baz() returns (l: bool)
+{
+  call l := bar();
+}
+
 procedure A1() 
 modifies g;
 {
@@ -33,4 +38,23 @@ modifies g;
 {
     g := true;
     assert |{ var l: bool; A: call l := bar(); return !l; }|;
+}
+
+procedure A5() 
+modifies g;
+{
+    var m: bool;
+
+    g := true;
+    m := |{ var l: bool; A: call l := bar(); return l; }|;
+    assert m;
+}
+
+procedure A6() 
+modifies g;
+{
+    g := true;
+    assert |{ var l: bool; A: call l := baz(); return l; }|;
+    assert (exists p: bool :: |{ var l: bool; A: call l := baz(); return l; }|);
+    assert (forall p: bool :: |{ var l: bool; A: call l := baz(); return l; }|);
 }
